start with chap1 of David Marker

chap1Script.sml
@@ -58,7 +58,7 @@ val _ = Datatype‘
              Pred : num -> α list -> bool |>
 ’;       
 
-Definition struc:
+Definition struc_def:
   struc L (M :α model) <=> (M.Dom <> {}) /\
   (!f nf. L.Fun_sym f nf ==>
           !as. LENGTH as = nf ==> (M.Fun f as) IN M.Dom) /\
@@ -67,7 +67,7 @@ Definition struc:
                !a. MEM a as ==> a IN M.Dom)
 End      
 
-Definition embed:
+Definition embed_def:
   embed L eta M N <=>
   (!f nf. L.Fun_sym f nf ==>
           !as. (LENGTH as = nf /\ 
@@ -79,7 +79,7 @@ Definition embed:
                M.Pred r as = N.Pred r (MAP eta as))
 End
 
-Definition substruc:
+Definition substruc_def:
   substruc L M N <=> struc L M /\ struc L N /\ M.Dom ⊆ N.Dom /\
                      embed L (\a. a) M N
 End        
@@ -95,14 +95,105 @@ Definition satis_def:
   satis M v ϕ <=> valuation M v /\ holds M v ϕ
 End
 
+Definition L_term_def:
+  L_term L t <=> (!f nf. (f, nf) IN (term_functions t) ==> L.Fun_sym f nf)
+End        
+
 Definition L_form_def:
   L_form L ϕ <=> (!f nf. (f, nf) IN (form_functions ϕ) ==> L.Fun_sym f nf) /\                    (!r nr. (r, nr) IN (form_predicates ϕ) ==> L.Pred_sym r nr)
 End
+
+Theorem L_term_MEM:
+  L_term L (Fn n l) /\ MEM x l ==> L_term L x
+Proof
+  rw[L_term_def] >> first_x_assum irule >>
+  ‘∃s. MEM s (MAP (λa. term_functions a) l) ∧ (f,nf') ∈ s’
+    suffices_by metis_tac[] >>
+  qexists_tac ‘term_functions x’ >> rw[MEM_MAP] >>
+  qexists_tac ‘x’ >> rw[]
+QED
+
+Theorem L_term_termval_in_Dom:
+  !t. L_term L t /\ struc L M /\ valuation M v ==> (termval M v t) IN M.Dom
+Proof
+completeInduct_on ‘term_size t’ >> Cases_on ‘t’ >> rw[termval_def] (* 2 *)
+>- fs[valuation_def] >>
+fs[struc_def] >> last_x_assum irule >> fs[L_term_def]
+QED       
                   
 Theorem prop_1_1_8_i:
-  substruc L M N /\ qfree ϕ /\  ==>
-  
-  
+  !t. substruc L M N /\ L_term L t /\ valuation M v ==>
+  termval M v t = termval N v t
+Proof
+completeInduct_on ‘term_size t’ >> rw[] >> Cases_on ‘t’ >> rw[termval_def] >>
+fs[substruc_def,embed_def] >>
+‘(MAP (λa. termval M v a) l) = (MAP (λa. termval N v a) l)’
+  by
+   (irule MAP_CONG >> rw[] >> first_x_assum irule >> rw[] (* 2 *)
+    >- (drule term_size_lemma >> strip_tac >>
+    ‘term_size x < 1 + (n + term1_size l)’ by metis_tac[] >>
+    fs[]) >>
+    metis_tac[L_term_MEM]) >>
+rw[] >> first_x_assum irule >> rw[] (* 2 *)
+>- (fs[MEM_MAP] >> fs[MAP_EQ_f] >> first_x_assum drule >> rw[] >>
+   ‘termval M v a' ∈ M.Dom’ suffices_by metis_tac[] >>
+   irule L_term_termval_in_Dom >> rw[] >>
+   qexists_tac ‘L’ >> rw[] >>
+   metis_tac[L_term_MEM]) >>
+fs[L_term_def,term_functions_def]
+QED
+
+Theorem substruc_valuation:
+  substruc L M N /\ valuation M v ==> valuation N v
+Proof
+rw[substruc_def,valuation_def,SUBSET_DEF]
+QED    
+
+Theorem L_term_Pred_MEM:
+  L_form L (Pred n l) /\ MEM x l ==> L_term L x
+Proof
+  rw[L_term_def,L_form_def,PULL_EXISTS] >> first_x_assum irule >>
+  qexists_tac ‘term_functions x’ >> rw[MEM_MAP] >>
+  qexists_tac ‘x’ >> rw[]
+QED
+
+Theorem L_form_IMP:
+  L_form L (IMP ϕ1 ϕ2) ==> L_form L ϕ1 /\ L_form L ϕ2
+Proof
+rw[L_form_def]
+QED
+       
+Theorem prop_1_1_8_ii:
+  !ϕ v. substruc L M N /\ L_form L ϕ /\ qfree ϕ /\ valuation M v ==>
+        satis M v ϕ = satis N v ϕ
+Proof
+Induct_on ‘ϕ’ >> rw[satis_def,qfree_def,holds_def] (* 2 *)
+>- (‘valuation N v’ by metis_tac[substruc_valuation] >> rw[] >>
+   fs[substruc_def,embed_def] >>
+   ‘MAP (termval M v) l = MAP (termval N v) l’
+     by
+      (irule MAP_CONG >> rw[] >>
+      ‘L_term L x’ by metis_tac[L_term_Pred_MEM] >> irule prop_1_1_8_i >>
+      rw[substruc_def,embed_def] >> qexists_tac ‘L’ >> rw[]) >>
+   rw[] >> first_x_assum irule >> rw[] (* 2 *)
+   >- (fs[MEM_MAP,MAP_EQ_f] >>
+      ‘termval M v y ∈ M.Dom’ suffices_by metis_tac[] >>
+      irule L_term_termval_in_Dom >> rw[] >> qexists_tac ‘L’ >> rw[] >>
+      metis_tac[L_term_Pred_MEM]) >>
+   fs[L_form_def]) >>
+‘valuation N v’ by metis_tac[substruc_valuation] >> rw[] >>
+drule L_form_IMP >> strip_tac >> metis_tac[satis_def]
+QED
+
+Definition sen_def:
+  sen ϕ <=> FV ϕ = {}
+End          
+
+Definition elem_equiv_def:
+elem_equiv L M N <=> struc L M /\ struc L N /\
+                     (!ϕ v. L_form L ϕ /\ sen ϕ /\ valuation M v ==>
+                            satis M v ϕ = satis N v ϕ)       
+End  
            
 
 val _ = export_theory();
